\documentclass[11pt, fullpage]{article}
\usepackage{graphicx, , mathtools, latexsym, amsfonts, amsmath, setspace, stmaryrd,amssymb}
\usepackage[margin = 2.5cm]{geometry}
\def\Var{{\rm Var}\,}
\def\Cov{{\rm Cov}\,}
\newcommand{\qed}{\mbox{\rule{.07in}{.07in}}}
\newcommand{\rdb}{\right\rrbracket}
\newcommand{\ldb}{\left\llbracket}
\newcommand{\db}[1]{\ldb #1 \rdb}
\newcommand{\ssum}{\sum\limits}
\newcommand{\pprod}{\prod\limits}
\newcommand{\mc}[2]{\left({ #1 \choose #2 } \right) }
\newcommand{\s}{\sigma}
\newcommand{\E}{\exists\hspace{1mm}}
\newcommand{\Aut}{\text{Aut}}
\newcommand{\iso}{\overset\sim\to}
\newcommand{\Gal}{\text{Gal}}
\newcommand{\arrow}{\longrightarrow}
\newcommand{\Spl}{\text{Spl}}
\newcommand{\triq}{\trianglelefteq}
\newcommand{\Hom}{\text{Hom}}
\newcommand{\tr}{\text{tr}}
\begin{document}
\begin{flushright}
Wyatt Alt\\
1/31/2013\\
\end{flushright}
\begin{flushleft}
\textbf{MCM HEAT}\\
\end{flushleft}
This will be a two step problem.  First I'll solve heat for the batter with unknown boundary conditions on the sides, then I'll solve it for the pan to derive those boundary conditions.
\begin{enumerate}
\item[1.] Consider a rectangular mass of batter flush with the first octant and having width $W$, height $H$, and depth $l$.  Let the width of the baking pan be $D$.  Let $K$ be the conduction constant for brownie batter.  Let $T_i$ be the initial temperature of the batter and let $T_b$ be the baking temperature.  Let $f$ be the heat function for the brownie pan, let $r = (x,y,z)$ and $s = x+D,y+D,z+D$.   We wish to find the a function $T$ satisfying
\[\partial{T}{t} = K \nabla^2 T\]
subject to the initial condition
\[T(x,y,z,0) = T_i\]
and boundary conditions \begin{align*}
T(0,y,z,t) = T(W,y,z,t) &= f(s,t)\\
T(x,0,z,t) = T(x,L,z,t) &= f(s,t)\\
T(x,y,0,t) &= f(s,t)\\
T(x,y,H,t) &= T_b \end{align*}
where $s$ modifies the coordinates on the term to the left.
To simplify the following computations, define
\[u(r,t) = T(r,t) - f(s,t)\]
The equation becomes 
\[\frac{\partial u}{\partial t} K \nabla^2 u\]
with initial condition
\[u(r,0) = T_i - f(s,t)\]
and boundary conditions \begin{align*}
T(0,y,z,t) = T(W,y,z,t) &= 0\\
T(x,0,z,t) = T(x,L,z,t) &= 0\\
T(x,y,0,t) &= 0\\
T(x,y,H,t) &= T_b\end{align*}
We get away with not subtracting from the last equation because the top of the batter is not exposed to the pan.\\
\\
Approaching this by separation of variables, suppose
\[u(r,t) = XYZG\]
where $X,Y,Z$, and $G$ are functions of $x,y,z$, and $t$.  We find that \begin{align*}
u_t &= XYZG'\\
u_{xx} &= X''YZG\\
u_{yy} &= XY''ZG\\
u_{zz} &= XYZ''G \end{align*}
Plugging these into the heat equation and dividing by $KXYZG$, we find \begin{align*}
XYZG' &= K(X''YZG +XyY'ZG + XYZ''G)\\
\implies \frac{G'}{KG}  = \frac{X''}{X} + \frac{Y''}{Y} + \frac{Z''}{Z} \end{align*}
note that the left hand side of this equation is constant, so the right must be as well.  Introducing $\lambda^2$, we write
\[\frac{G'}{KG} = -\lambda^2 \hspace{15mm} \frac{X''}{X} + \frac{Y''}{Y} + \frac{Z''}{Z} = -\lambda^2\]
From the first equation, we immediately get the ODE
\[G'-G\lambda^2 = 0\]
For the other, let
\[\frac{X''}{X} = -\frac{Y''}{Y} - \frac{Z''}{Z} - \lambda^2 = -\mu^2\]
then 
\[\frac{Y''}{Y} = -\frac{Z''}{Z} - \lambda^2 + \mu^2 = -\nu^2\]
and
\[\frac{Z''}{Z} = - \lambda^2 + \mu^2 + \nu^2 = -\rho^2\]
\\
We can now derive the following equations: \begin{align*}
X''+ \mu^2 X &= 0\\
Y'' + \nu^2 Y &= 0\\
Z'' + \rho^2 Z &= 0 
\lambda^2 &= \mu^2 + \nu^2 + \rho^2
\intertext{and the one from before}
G'-G\lambda^2 = 0 \end{align*}
The general solution $G$ is $G = A e^{-\lambda^2 K t}$ for some constant $A$.  The general solution for $X'' + \mu^2 X = 0$ is 
\[X = c_1 \cos \mu x + c_2 \sin \mu x\]
Considering the boundary condition $X(0) = 0$, note that $c_1 = 0$.  Considering $X(W) = 0$, we must have $c_2 \sin \mu W = 0$.  Since $c_2=0$ is a trivial case, we focus on cases where $\sin \mu W = 0$.  This happens when $\mu W$ is an integer multiple of $\pi$.  We note therefore that
\[\mu_m = \frac{m \pi}{W}\]
for $m = 1,2, \dots$.  Substituting these findings into the equation for $X$, we find solutions
\[X_m(x) = \sin(\frac{m \pi x}{W})\]
the same method leads to a solution for $Y$:
\[Y_n(y) = \sin(\frac{n \pi y}{L})\]
for $n = 1,2,\dots$.\\
For $Z$, the boundary conditions are $Z(0) = 0$ and $Z(H) = T_b$ so we let
\[Z = \gamma_l e^{\rho_l z} + \delta_l e^{-\rho_l z}\]
the boundary condition $Z(0) = 0$ gives us $\gamma_l = -\delta_l$.  Choosing $\gamma_l = \frac{1}{2}$ we find
\[Z_l(z) = \sinh \rho_l z\]
the separated solution for $u$ is thus
\[u_{mnl}(r,t) = A_{mnl} \sin(\mu_m x) \sin (\nu_n y) \sinh (\rho_l z) e^{-\lambda^2_{mnl}Kt}\]
with
\[\lambda_{mnl}^2 = \mu_m^2 + \nu_n^2 + \rho_l^2 = \left(\frac{m \pi}{W}\right)^2 + \left(\frac{n \pi}{L} \right)^2 + \left(\frac{l \pi}{H}\right)^2\]
for $m,n,l = 1,2 \dots$\\
We can also form a linear superposition:
\[u(r,t) = \ssum_{m=1}^\infty \ssum_{n=1}^\infty \ssum_{l=1}^\infty A_{mnl} \sin(\mu_m x) \sin (\nu_n y) \sinh (\rho_l z) e^{-\lambda^2_{mnl}Kt}\]
with constants $A_{mnl}$.  This general solution satisfies the boundary conditions on all sides except the top.  To determine the values of the constants $A_{mnl}$, note the initial condition
\[u(r,0) = T_i - f(s,0)\]
we find
\[T_i - f(s,0) = \ssum_{m,=1}^\infty \ssum_{n=1}^\infty \ssum_{l=1}^\infty A_{mnl} \sin(\mu_m x) \sin (\nu_n y) \sinh (\rho_l z) \]
Let 
\[b_m(y,z) = \ssum_{n=1}^\infty \ssum_{l=1}^\infty A_{mnl} \sin (\nu_n y) \sinh (\rho_l z)\]
and consider that 
\[T_i - f(s,0) = \ssum_{m=1}^\infty b_m(y,z) \sin (\mu_m x)\]
we multiply both sides by $\sin (\mu_k x)$ and integrate, interchanging the integral and sum on the left: \begin{align*}
\int_0^W (T_i - f(s,0)) \sin(\mu_k x) dx &= \ssum_{m=1}^\infty \int_0^W b_m(y,z) \sin(\mu_m x) \sin (\mu_k x) dx
\intertext{Take note that on the right hand side, the sines are orthogonal unless $k = m$, leaving}
\int_0^W (T_i - f(s,0)) \sin(\mu_m x) dx &= \int_0^W b_m(y,z) \sin(\mu_m x) \sin (\mu_k x)
&= \frac{b_m(y,z) W}{2}\\
\end{align*}
and so we have 
\[b_m(y,z) = \frac{2}{W} \int_0^W (T_i - f(s,0)) \sin(\mu_m x) dx\]
the same technique will produce the analogous
\[c_n(x,z) = \frac{2}{L} \int_0^L (T_i - f(s,0)) \sin(\mu_n y) dy\]
for the opposite side. In the vertical direction, we let
\[d_l(x,y) = \ssum_{m=1}^\infty \ssum_{n=1}^\infty \sin(\mu_m x) \sin (\nu n y)\]
and so \begin{align*}
T_i - f(s,0) &= \ssum_{l=1}^\infty d_l(x,y) \sinh (\rho_l z)\\
&= \ssum_{l=1}^\infty d_l(x,y) \dfrac{e^{\rho_l z} - e^{-\rho_l z}}{2}\\
&= \frac{1}{2} \ssum_{l=1}^\infty d_l(x,y) (e^{\rho_l z} - e^{-\rho_l z})\\
2(T_i - f(s,0)) &= \ssum_{l=1}^\infty d_l (x,y) e^{\rho_l z} - \ssum_{l=1}^\infty d_l(x,y) e^{-\rho_l z} \end{align*}
let 
\[\delta(r) = \ssum_{l=1}^\infty d_l(x,y) e^{\rho_l z}\]
and 
\[\gamma(r) = \ssum_{l=1}^\infty d_l(x,y) e^{-\rho_l z}\]
Then
\[2(T_i - f(s,0)) = \delta(r) - \gamma(r)\]
and by fourier series,
\[d_n = \frac{2}{H} \int_0^H \delta(r) e^{-\rho_l z} dz = \frac{2}{H} \int_0^H \gamma(r) e^{\rho_l z} dz\]

\end{enumerate}
\end{document}